% \begin{tabbing}
%   % \begin{align*}
%   {\sc CoreChoices}$\ :\ C \rightarrow vm \rightarrow ev \rightarrow vm$ \\
%   {\sc CoreChoices}$\ C\ mdls\ v$\\
%   \qquad case $v$ of \\
%   \qquad \qquad \= Unit \qquad \qquad \= = return \mdls{} \\
%   \> \chc[d]{e,e'} \> = CoreChoicesHelper C \dimd{} \mdls{} (Evaluate e) (Evaluate e') \\
%   \> \chc[d]{e,e'} $\wedge\ ev\ $ \> = do \\
%   \> \> \quad \=  $vE \leftarrow$ Evaluate $e$ \\
%   \> \> \> $vE' \leftarrow$ Evaluate $e'$ \\
%   \> \> \> CoreChoicesHelper C \dimd{} \mdls{} ($vE \wedge\ ev$) ($vE' \wedge ev$) \\
%   \> $ev\ \wedge\ $\chc[d]{e,e'} \> = do \\
%   \> \> \quad \=  $vE \leftarrow$ Evaluate $e$ \\
%   \> \> \> $vE' \leftarrow$ Evaluate $e'$ \\
%   \> \> \> CoreChoicesHelper C \dimd{} \mdls{} ($ev \wedge\ vE$) ($ev \wedge eV'$) \\
%   \> \chc[d]{e,e'} $\vee\ ev\ $ \> = do \\
%   \> \> \quad \=  $vE \leftarrow$ Evaluate $e$ \\
%   \> \> \> $vE' \leftarrow$ Evaluate $e'$ \\
%   \> \> \> CoreChoicesHelper C \dimd{} \mdls{} ($vE \vee\ ev$) ($vE' \vee ev$) \\
%   \> $ev\ \vee\ $\chc[d]{e,e'} \> = do \\
%   \> \> \quad \=  $vE \leftarrow$ Evaluate $e$ \\
%   \> \> \> $vE' \leftarrow$ Evaluate $e'$ \\
%   \> \> \> CoreChoicesHelper C \dimd{} \mdls{} ($ev \vee\ vE$) ($ev \vee eV'$) \\
%   \> $ev$ \> = do \\
%   \> \> \quad \= $vE \leftarrow$ FindPChoice (Evaluate $ev$) \\
%   \> \> \> solveChoices C \dimd{} \mdls{} ($vE$)  \\
% \end{tabbing}
\begin{mathpar}
  %%% Computation rules
  \inferrule*[Right=Gen-M]
  { \texttt{genModel($\Phi$)} = m }
  { (\Phi, \unit{}) \Downarrow_{i} m }

  \inferrule*[Right=Cr-Sym]
  { ((\Gamma, \Delta), s) \rightarrowtail ((\Gamma', \Delta'), \unit{})}
  { ((C, \Gamma, \Delta), s) \Downarrow_{i} ((C, \Gamma', \Delta'), \unit{})
  }
\end{mathpar}
%
\begin{mathpar}
\inferrule*[Right=Cr-And]
{ (\Phi, v_{1}) \Downarrow_{i} (\Phi_{1}, v_{1}') \\
    (\Phi_1, v_{2}) \Downarrow_{1} (\Phi', v_{2}') \\
  }
  { (\Phi, v_{1} \wedge v_{2}) \Downarrow_{i} (\Phi', v_{1}' \wedge v_{2}')
  }
\\%
%   \hspace{0.5cm}
  %% solve a symbolic reference execute
  \inferrule*[Right=Cr-Or]
  { (\Delta, v_{1} \vee v_{2}) \mapsto (\Delta', v)}
  { ((C, \Gamma, \Delta), v_{1} \vee v_{2}) \Downarrow_{i} ((C, \Gamma, \Delta'), v) }

\\%
%%%%%%% And rules %%%%%%%%%%%%%%%%%%%%%
\inferrule*[Right=Cr-And-TR]
{
  C(D) = \true \\
  ((C, \Gamma, \Delta), v \wedge \texttt{toIR$(e_{1})$}) \Downarrow_{i} m
}
{
  ((C, \Gamma, \Delta), v \wedge \chc[D]{e_{1}, e_{2}}) \Downarrow_{i} m
}
\\
\inferrule*[Right=Cr-And-TL]
{
  C(D) = \true \\
  ((C, \Gamma, \Delta), \texttt{toIR$(e_{1})$} \wedge v) \Downarrow_{i} m
}
{
  ((C, \Gamma, \Delta), \chc[D]{e_{1}, e_{2}} \wedge v) \Downarrow_{i} m
}

\\%
\inferrule*[Right=Cr-And-FR]
{
  C(D) = \false \\
  ((C, \Gamma, \Delta), v \wedge \texttt{toIR$(e_{2})$}) \Downarrow_{i} m
}
{
  ((C, \Gamma, \Delta), v \wedge \chc[D]{e_{1}, e_{2}}) \Downarrow_{i} m
}
\\
\inferrule*[Right=Cr-And-FL]
{
  C(D) = \false \\
  ((C, \Gamma, \Delta), \texttt{toIR$(e_{2})$} \wedge v) \Downarrow_{i} m
}
{
  ((C, \Gamma, \Delta), \chc[D]{e_{1}, e_{2}} \wedge v) \Downarrow_{i} m
}

%%%%%%%%%%%%%%%%%%%%%%%% Or rules %%%%%%%%%%%%%%%%%%%%%%%%%%%%%%%%%%%

\inferrule*[Right=Cr-Or-TR]
{
  C(D) = \true \\
  ((C, \Gamma, \Delta), v \vee \texttt{toIR$(e_{1})$}) \Downarrow_{i} m
}
{
  ((C, \Gamma, \Delta), v \vee \chc[D]{e_{1}, e_{2}}) \Downarrow_{i} m
}
\\
\inferrule*[Right=Cr-Or-TL]
{
  C(D) = \true \\
  ((C, \Gamma, \Delta), \texttt{toIR$(e_{1})$} \vee v) \Downarrow_{i} m
}
{
  ((C, \Gamma, \Delta), \chc[D]{e_{1}, e_{2}} \vee v) \Downarrow_{i} m
}

\\%
\inferrule*[Right=Cr-Or-FR]
{
  C(D) = \false \\
  ((C, \Gamma, \Delta), v \vee \texttt{toIR$(e_{2})$}) \Downarrow_{i} m
}
{
  ((C, \Gamma, \Delta), v \vee \chc[D]{e_{1}, e_{2}}) \Downarrow_{i} m
}
\\
\inferrule*[Right=Cr-Or-FL]
{
  C(D) = \false \\
  ((C, \Gamma, \Delta), \texttt{toIR$(e_{2})$} \vee v) \Downarrow_{i} m
}
{
  ((C, \Gamma, \Delta), \chc[D]{e_{1}, e_{2}} \vee v) \Downarrow_{i} m
}


%%%%%%%%%%%%%%%%%%%%%%%%%%%%%%%% Choice rules %%%%%%%%%%%%%%%%%%%%%%%%%%%%%%%%%%
  \inferrule*[Right=Cr-CAnd-R]
  {
    \hspace{1.3cm}
    ((C \cup \{(D, \true)\}, \Gamma, \Delta), v \wedge \chc[D]{e_{1}, e_{2}}) \Downarrow_{i+1} m_{1} \\
    D \notin C \\
    ((C \cup \{(D, \false)\}, \Gamma, \Delta), v \wedge \chc[D]{e_{1}, e_{2}}) \Downarrow_{i+1} m_{2} \\
  }
  {
    ((C, \Gamma, \Delta), v \wedge \chc[D]{e_{1}, e_{2}}) \Downarrow_{i} m_{1}
    \oplus m_{2}
  }
  \\
  \inferrule*[Right=Cr-COr-R]
  {
    \hspace{1.3cm}
    ((C \cup \{(D, \true)\}, \Gamma, \Delta), v \vee \chc[D]{e_{1}, e_{2}}) \Downarrow_{i+1} m_{1} \\
    D \notin C \\
    ((C \cup \{(D, \false)\}, \Gamma, \Delta), v \vee \chc[D]{e_{1}, e_{2}}) \Downarrow_{i+1} m_{2} \\
  }
  {
    ((C, \Gamma, \Delta), v \vee \chc[D]{e_{1}, e_{2}}) \Downarrow_{i} m_{1}
    \oplus m_{2}
  }
  \\

  \inferrule*[Right=Cr-CAnd-L]
  {
    \hspace{1.3cm}
    ((C \cup \{(D, \true)\}, \Gamma, \Delta), \chc[D]{e_{1}, e_{2}} \wedge v) \Downarrow_{i+1} m_{1} \\
    D \notin C \\
    ((C \cup \{(D, \false)\}, \Gamma, \Delta), \chc[D]{e_{1}, e_{2}} \wedge v) \Downarrow_{i+1} m_{2} \\
  }
  {
    ((C, \Gamma, \Delta), \chc[D]{e_{1}, e_{2}} \wedge v) \Downarrow_{i} m_{1}
    \oplus m_{2}
  }
  \\
  \inferrule*[Right=Cr-COr-L]
  {
    \hspace{1.3cm}
    ((C \cup \{(D, \true)\}, \Gamma, \Delta), \chc[D]{e_{1}, e_{2}} \vee v) \Downarrow_{i+1} m_{1} \\
    D \notin C \\
    ((C \cup \{(D, \false)\}, \Gamma, \Delta), \chc[D]{e_{1}, e_{2}} \vee v) \Downarrow_{i+1} m_{2} \\
  }
  {
    ((C, \Gamma, \Delta), \chc[D]{e_{1}, e_{2}} \vee v) \Downarrow_{i} m_{1}
    \oplus m_{2}
  }
%
\end{mathpar}
