\begin{mathpar}
  %%% Computation rules
  \inferrule*[Right=Ev-Term]
  { \texttt{assert($(\Gamma, \Delta), t$)} = \Gamma' }
  {((\Gamma, \Delta), t) \rightarrowtail ((\Gamma', \Delta), \unit{}) }
\\
  \inferrule*[Right=Ev-Sym]
  { \texttt{assert($(\Gamma, \Delta), s$)} = \Gamma'}
  { ((\Gamma, \Delta), s) \rightarrowtail ((\Gamma', \Delta), \unit{}) }
\\
  \inferrule*[Right=Ev-Chc]
  { }
  {(\Theta, \chc[D]{e_{1}, e_{2}}) \rightarrowtail (\Theta, \chc[D]{e_{1}, e_{2}})}
%
%   \hspace{0.5cm}
%   \inferrule*[Right=Ev-Unit]
%   { }
%   { (\Theta,\unit{}) \rightarrowtail (\Theta, \unit{}) }
\\
  %%%\unit{} elimination rules
  \inferrule*[Right=Ev-UL]
  {  }
  { (\Theta,\unit{} \wedge v) \rightarrowtail (\Theta, v) }

  \inferrule*[Right=Ev-UR]
  { }
  { (\Theta, v \wedge\unit{}) \rightarrowtail (\Theta, v)}

\\

  \inferrule*[Right=Ev-DM-VOr]
  { }
  { (\Theta, \neg (v_{1} \vee v_{2})) \rightarrowtail (\Theta ,\neg v_{1} \wedge \neg v_{2})}
\\
  \inferrule*[Right=Ev-DM-VAnd]
  { }
  { (\Theta, \neg (v_{1} \wedge v_{2})) \rightarrowtail (\Theta, \neg v_{1} \vee \neg v_{2})}

  %%% Negation rules
  % \inferrule*[Right=Ev-NegS]
  % { (\Delta, \neg s) \mapsto (\Delta', s') \\
  %   ((\Gamma, \Delta'), s') \rightarrowtail (\Theta, \unit{})
  % }
  % { ((\Gamma, \Delta), \neg s) \rightarrowtail (\Theta, \unit{})}
\\
%   \inferrule*[Right=Ev-Neg-Chc]
%   { }
%   { (\Theta, \neg \chc[D]{e_{1},e_{2}}) \rightarrowtail (\Theta, \chc[D]{\neg e_{1}, \neg e_{2}}) }

  \inferrule*[Right=Ev-Neg]
  { (\Delta,\neg v) \mapsto (\Delta', v')
    % ((\Gamma, \Delta') ,\neg v) \rightarrowtail (\Theta, v')
  }
  { ((\Gamma, \Delta), \neg v) \rightarrowtail ((\Gamma, \Delta'), v') }
  \\
  %%% And with Choice rules
% \begin{mathpar}
%   \hspace{-1.5cm}
%   \inferrule*[Right=Ev-And-ChcL]
%   { \Gamma, \Delta,e \rightarrowtail \Gamma', \Delta',e'}
%   { \Gamma, \Delta,\chc[D]{e_{1},e_{2}} \wedge e \rightarrowtail \Gamma',
%     \Delta',\chc[D]{e_{1},e_{2}} \wedge e' }
% \end{mathpar}
% \begin{mathpar}
%   \hspace{-1.5cm}
%   \inferrule*[Right=Ev-And-ChcR]
%   { \Gamma, \Delta,e \rightarrowtail \Gamma', \Delta',e'}
%   { \Gamma, \Delta,e \wedge \chc[D]{e_{1},e_{2}} \rightarrowtail \Gamma',
%     \Delta',e' \wedge \chc[D]{e_{1},e_{2}} }
%   % {l \rightarrowtail l'}
%   % { l \wedge \chc[D]{e_{1},e_{2}} \rightarrowtail l' \wedge \chc[D]{e_{1},e_{2}}}
% \end{mathpar}
%   %%% Or with Choice rules
% \begin{mathpar}
%   \hspace{-1.5cm}
%   \inferrule*[Right=Ev-Or-ChcL]
%   {\Delta,e \mapsto \Delta',v}
%   { \Gamma, \Delta,\chc[D]{e_{1},e_{2}} \vee e \rightarrowtail \Gamma,
%     \Delta',\chc[D]{e_{1},e_{2}} \vee v}
% \end{mathpar}
% \begin{mathpar}
%   \hspace{-1.5cm}
%   \inferrule*[Right=Ev-Or-ChcR]
%   {\Delta,e \mapsto \Delta',v}
%   { \Gamma, \Delta,e \vee \chc[D]{e_{1},e_{2}} \rightarrowtail \Gamma,
%     \Delta',v \vee \chc[D]{e_{1},e_{2}} }
% \end{mathpar}
% \begin{mathpar% }
%   \inferrule*[Right=Ev-Or-Value]
%   {(\Delta, e_{1}) \mapsto (\Delta_{1}, s_{1}) \\
%     (\Delta_{1}, e_{2}) \mapsto (\Delta_{2}, s_{2}) \\
%     (\Delta_{2}, s_{1} \vee s_{2}) \mapsto (\Delta_{s}, s) \\
%     ((\Gamma, \Delta_{s}), s) \twoheadrightarrow (\Theta,\unit{})
%   }
%   { ((\Gamma, \Delta),e_{1} \vee e_{2}) \rightarrowtail (\Theta,\unit{})}
% \end{mathpar}
  %%% Congruence rules with symbolic execution
  \inferrule*[Right=Ev-Or]
  { (\Delta, v_{1}) \mapsto (\Delta_{1}, v_{1}) \\
    (\Delta_{1},v_{2}) \mapsto (\Delta', v_{2})}
  { ((\Gamma, \Delta), v_{1} \vee v_{2}) \rightarrowtail ((\Gamma, \Delta'), v_{1}' \vee v_{2}')}

  \inferrule*[Right=Ev-And]
  {(\Theta, v_{1}) \rightarrowtail (\Theta_{1}, v_{1}') \\
    (\Theta_{1}, v_{2}) \rightarrowtail (\Theta', v_{2}')
  }
  { (\Theta, v_{1} \wedge v_{2}) \rightarrowtail (\Theta', v_{1}' \wedge v_{2}')
  }
\end{mathpar}%
